Neighborhood/Semantics/Logic/ECP.lean
@@ -1,0 +1,40 @@
+module
+
+public import Neighborhood.Semantics.Logic.E
+public import Neighborhood.Semantics.Logic.ECD
+public import Neighborhood.Semantics.Example.Frame1_1
+
+@[expose] public section
+
+variable {α : Type u} {A : Formula α}
+
+
+theorem LogicECP.sound {κ} [Nonempty κ] (F : Frame κ) [F.IsRegular] [F.NotContainsEmpty] :
+    A ∈ LogicECP → F ⊧ A :=
+  Hilbert.sound (by rintro _ (⟨_, _, rfl⟩ | rfl) <;> simp)
+
+theorem LogicECP.consistent : (@LogicECP α).IsConsistent := by
+  by_contra! hC
+  simpa using LogicECP.sound frame_1_2 hC
+
+instance : Nonempty (MaximalConsistentSet (@LogicECP α)) :=
+  MaximalConsistentSet.nonempty LogicECP.consistent
+
+variable [DecidableEq α]
+
+theorem LogicECP.complete
+    (h : ∀ {κ : Type u} [Nonempty κ] (F : Frame κ), [F.IsRegular] → [F.NotContainsEmpty] → F ⊧ A) :
+    A ∈ @LogicECP α :=
+  (basicCanonicity LogicECP).mem_of_valid
+    (h (basicCanonicity LogicECP).toModel.toFrame
+      (basicCanonicity LogicECP).toModel.Val)
+
+theorem LogicECD_ssubset_LogicECP : @LogicECD ℕ ⊂ LogicECP := by
+  constructor
+  · apply Hilbert.subset_of_provable_axioms
+    rintro A (⟨B, C, rfl⟩ | ⟨B, rfl⟩) <;> first | exact Logic.axiomC | exact Logic.axiomD
+  · intro h
+    have hP : (Axioms.P : Formula ℕ) ∈ @LogicECD ℕ := h (ProvableHilbert.axm (by grind))
+    exact frame_1_1.not_valid_axiomP (LogicECD.sound frame_1_1 hP)
+
+end
