Neighborhood/Semantics/Logic/EMD.lean
@@ -1,9 +1,13 @@
 module
 
+public import Neighborhood.Semantics.Logic.E
 public import Neighborhood.Semantics.Logic.ED
 public import Neighborhood.Semantics.Logic.EM
+public import Neighborhood.Semantics.Logic.EMP
+public import Neighborhood.Semantics.Supplementation
 public import Neighborhood.Semantics.Example.Frame1_1
 public import Neighborhood.Semantics.Example.Frame1_3
+public import Neighborhood.Semantics.Example.Frame2_238
 
 /-!
 # The neighborhood logic `LogicEMD`
@@ -32,6 +36,13 @@ theorem consistent : (@LogicEMD α).IsConsistent := by
 instance : Nonempty (MaximalConsistentSet (@LogicEMD α)) :=
   MaximalConsistentSet.nonempty LogicEMD.consistent
 
+theorem complete
+    (h : ∀ {κ : Type u} [Nonempty κ] (F : Frame κ), [F.IsMonotonic] → [F.IsSerial] → F ⊧ A) :
+    A ∈ @LogicEMD α :=
+  (supplementedBasicCanonicity LogicEMD).mem_of_valid
+    (h (supplementedBasicCanonicity LogicEMD).toModel.toFrame
+      (supplementedBasicCanonicity LogicEMD).toModel.Val)
+
 end LogicEMD
 
 theorem LogicED_ssubset_LogicEMD : @LogicED ℕ ⊂ LogicEMD := by
@@ -47,5 +58,13 @@ theorem LogicEM_ssubset_LogicEMD : @LogicEM ℕ ⊂ LogicEMD := by
   · intro h
     have hD : Axioms.D #0 ∈ (@LogicEM ℕ) := h (ProvableHilbert.axm (by grind))
     exact frame_1_3.not_isSerial (isSerial_of_valid_axiomD (LogicEM.sound frame_1_3 hD))
+
+theorem LogicEMP_ssubset_LogicEMD : @LogicEMP ℕ ⊂ LogicEMD := by
+  constructor
+  · apply Hilbert.subset_of_provable_axioms
+    rintro A (⟨B, C, rfl⟩ | rfl) <;> first | exact Logic.axiomM | exact Logic.axiomP_of_MD
+  · intro h
+    have hD : Axioms.D #0 ∈ @LogicEMP ℕ := h (ProvableHilbert.axm (by grind))
+    exact frame_2_238.not_valid_axiomD (LogicEMP.sound frame_2_238 hD)
 
 end
