Neighborhood/Semantics/Logic/EMND.lean
@@ -1,10 +1,14 @@
 module
 
+public import Neighborhood.Semantics.Logic.E
 public import Neighborhood.Semantics.Logic.EMN
 public import Neighborhood.Semantics.Logic.EMD
+public import Neighborhood.Semantics.Logic.EMNP
+public import Neighborhood.Semantics.Supplementation
 public import Neighborhood.Semantics.Example.Frame1_3
 public import Neighborhood.Semantics.Example.Frame1_2
 public import Neighborhood.Semantics.Example.Frame1_0
+public import Neighborhood.Semantics.Example.Frame2_238
 
 /-!
 # The neighborhood logic `LogicEMND`
@@ -44,5 +48,28 @@ theorem LogicEMD_ssubset_LogicEMND : @LogicEMD ℕ ⊂ LogicEMND := by
   · intro h
     have hN : (Axioms.N : Formula ℕ) ∈ @LogicEMD ℕ := h (ProvableHilbert.axm (by grind))
     exact frame_1_0.not_valid_axiomN (LogicEMD.sound frame_1_0 hN)
+
+theorem LogicEMNP_ssubset_LogicEMND : @LogicEMNP ℕ ⊂ LogicEMND := by
+  constructor
+  · apply Hilbert.subset_of_provable_axioms
+    rintro A ((⟨B, C, rfl⟩ | rfl) | rfl) <;>
+      first | exact Logic.axiomM | exact Logic.axiomN | exact Logic.axiomP_of_ND
+  · intro h
+    have hD : Axioms.D #0 ∈ @LogicEMNP ℕ := h (ProvableHilbert.axm (by grind))
+    exact frame_2_238.not_valid_axiomD (LogicEMNP.sound frame_2_238 hD)
+
+section
+
+variable [DecidableEq α]
+
+theorem LogicEMND.complete
+    (h : ∀ {κ : Type u} [Nonempty κ] (F : Frame κ), [F.IsMonotonic] → [F.ContainsUnit] →
+      [F.IsSerial] → F ⊧ A) :
+    A ∈ @LogicEMND α :=
+  (supplementedBasicCanonicity LogicEMND).mem_of_valid
+    (h (supplementedBasicCanonicity LogicEMND).toModel.toFrame
+      (supplementedBasicCanonicity LogicEMND).toModel.Val)
+
+end
 
 end
