Neighborhood/Semantics/Logic/EMNP.lean
@@ -1,0 +1,33 @@
+module
+
+public import Neighborhood.Semantics.Logic.E
+public import Neighborhood.Semantics.Supplementation
+
+@[expose] public section
+
+variable {α : Type u} {A : Formula α}
+
+
+theorem LogicEMNP.sound {κ} [Nonempty κ] (F : Frame κ) [F.IsMonotonic] [F.ContainsUnit]
+    [F.NotContainsEmpty] :
+    A ∈ LogicEMNP → F ⊧ A :=
+  Hilbert.sound (by rintro _ ((⟨_, _, rfl⟩ | rfl) | rfl) <;> simp)
+
+theorem LogicEMNP.consistent : (@LogicEMNP α).IsConsistent := by
+  by_contra! hC
+  simpa using LogicEMNP.sound frame_1_2 hC
+
+instance : Nonempty (MaximalConsistentSet (@LogicEMNP α)) :=
+  MaximalConsistentSet.nonempty LogicEMNP.consistent
+
+variable [DecidableEq α]
+
+theorem LogicEMNP.complete
+    (h : ∀ {κ : Type u} [Nonempty κ] (F : Frame κ), [F.IsMonotonic] → [F.ContainsUnit] →
+      [F.NotContainsEmpty] → F ⊧ A) :
+    A ∈ @LogicEMNP α :=
+  (supplementedBasicCanonicity LogicEMNP).mem_of_valid
+    (h (supplementedBasicCanonicity LogicEMNP).toModel.toFrame
+      (supplementedBasicCanonicity LogicEMNP).toModel.Val)
+
+end
